Strata/Transform/DetToKleene.lean
@@ -1,0 +1,48 @@
+/-
+  Copyright Strata Contributors
+
+  SPDX-License-Identifier: Apache-2.0 OR MIT
+-/
+module
+
+public import Strata.DL.Imperative.Cmd
+public import Strata.DL.Imperative.Stmt
+public import Strata.DL.Imperative.KleeneStmt
+public import Strata.Languages.Core.StatementType
+
+/-! # Deterministic-to-Kleene Transformation -/
+
+public section
+
+open Imperative
+mutual
+
+/-- Deterministic-to-Kleene transformation for a single
+(deterministic) statement -/
+def StmtToKleeneStmt {P : PureExpr} [Imperative.HasBool P] [HasNot P]
+  (st : Imperative.Stmt P (Cmd P)) :
+  Imperative.KleeneStmt P (Cmd P) :=
+  match st with
+  | .cmd    cmd => .cmd cmd
+  | .block  _ bss _ => BlockToKleeneStmt bss
+  | .ite    cond tss ess md =>
+    .choice
+      (.seq (.assume "true_cond" cond md) (BlockToKleeneStmt tss))
+      (.seq ((.assume "false_cond" (Imperative.HasNot.not cond) md)) (BlockToKleeneStmt ess))
+  | .loop   guard _measure _inv bss md =>
+    .loop (.seq (.assume "guard" guard md) (BlockToKleeneStmt bss))
+  | .typeDecl _ md => (.assume "skip" Imperative.HasBool.tt md)
+  | .exit _ md => (.assume "skip" Imperative.HasBool.tt md)
+  | .funcDecl _ md => (.assume "skip" Imperative.HasBool.tt md)
+
+/-- Deterministic-to-Kleene transformation for multiple
+(deterministic) statements -/
+def BlockToKleeneStmt {P : Imperative.PureExpr} [Imperative.HasBool P] [HasNot P]
+  (ss : Imperative.Block P (Cmd P)) :
+  Imperative.KleeneStmt P (Cmd P) :=
+  match ss with
+  | [] => (.assume "skip" Imperative.HasBool.tt .empty)
+  | s :: ss => .seq (StmtToKleeneStmt s) (BlockToKleeneStmt ss)
+end
+
+end
