StrataTest/Transform/DetToKleene.lean
@@ -4,7 +4,7 @@
   SPDX-License-Identifier: Apache-2.0 OR MIT
 -/
 
-import Strata.Transform.DetToNondet
+import Strata.Transform.DetToKleene
 import Strata.Languages.Core.StatementSemantics
 import Strata.Languages.Core.ProgramType
 import Strata.Languages.Core.ProgramWF
@@ -12,25 +12,25 @@ import Strata.DL.Lambda.IntBoolFactory
 
 open Core
 
-/-! ## Deterministic-to-Nondeterministic Examples -/
-section NondetExamples
+/-! ## Deterministic-to-Kleene Examples -/
+section KleeneExamples
 
 open Imperative
 
-def NondetTest1 : Stmt Expression (Cmd Expression) :=
+def KleeneTest1 : Stmt Expression (Cmd Expression) :=
   .ite (Core.true) [.cmd $ .havoc "x" .empty ] [.cmd $ .havoc "y" .empty ] .empty
 
-def NondetTest1Ans : NondetStmt Expression (Cmd Expression) :=
+def KleeneTest1Ans : KleeneStmt Expression (Cmd Expression) :=
   .choice
     (.seq (.cmd (.assume "true_cond" Core.true .empty)) (.seq (.cmd $ .havoc "x" .empty) (.assume "skip" Imperative.HasBool.tt .empty)))
     (.seq (.cmd (.assume "false_cond" Core.false .empty)) (.seq (.cmd $ .havoc "y" .empty) (.assume "skip" Imperative.HasBool.tt .empty)))
 
 
--- #eval toString $ Std.format (StmtToNondetStmt NondetTest1)
--- #eval toString $ Std.format NondetTest1Ans
+-- #eval toString $ Std.format (StmtToKleeneStmt KleeneTest1)
+-- #eval toString $ Std.format KleeneTest1Ans
 
 /-- info: true -/
 #guard_msgs in
-#eval (toString $ Std.format (StmtToNondetStmt NondetTest1)) == (toString $ Std.format NondetTest1Ans)
+#eval (toString $ Std.format (StmtToKleeneStmt KleeneTest1)) == (toString $ Std.format KleeneTest1Ans)
 
-end NondetExamples
+end KleeneExamples
